src/tls/TLSInfo.fst
@@ -81,13 +81,13 @@ let defaultTicketCB = {
   new_ticket = defaultTicketCBFun;
 }
 
-val defaultServerNegoCBFun: server_nego_cb_fun
+val defaultServerNegoCBFun: nego_cb_fun
 let defaultServerNegoCBFun _ pv cext ocookie =
-  Nego_accept empty_bytes
+  Nego_accept []
 
-let defaultServerNegoCB : server_nego_cb = {
-  server_nego_context = FStar.Dyn.mkdyn ();
-  server_nego = defaultServerNegoCBFun;
+let defaultServerNegoCB : nego_cb = {
+  nego_context = FStar.Dyn.mkdyn ();
+  negotiate = defaultServerNegoCBFun;
 }
 
 let none4 = fun _ _ _ _ -> None
@@ -121,6 +121,7 @@ let defaultConfig =
   // Client
   hello_retry = true;
   offer_shares = [SEC CC.ECC_X25519];
+  custom_extensions = [];
 
   // Server
   check_client_version_in_pms_for_old_tls = true;
